examples/localise_globalise.thy
@@ -30,12 +30,6 @@ definition V3 where "V3 = (vu:d3 = sys:x \<and> (if sys:x < sys:y then (vu:e3 = 
 
 definition ExSys where "ExSys = (x\<^sup>> \<ge> 0 \<and> y\<^sup>> \<ge> 0 \<and> x\<^sup>> + y\<^sup>> = 10)\<^sub>e"
 
-(*
-definition ExSys_one_alpha where "ExSys_one_alpha = (sys:x \<ge> 0 \<and> sys:y \<ge> 0 \<and> sys:x + sys:y = 10)\<^sub>e"
-
-definition ExSys_two_delta where "ExSys_two_delta = (sys:x \<ge> 0 \<and> sys:y \<ge> 0 \<and> sys:x + sys:y = 10)\<^sub>e"
-*)
-
 lemma v1_healthy1: "V1 is VH1"
   by (pred_auto_banks add: V1_def)
 
@@ -48,56 +42,32 @@ lemma v3_healthy1: "V3 is VH1"
 definition Loc1 where "Loc1 = L V1 ExSys"
 
 lemma localise_v1 : "Loc1 = (a1 \<ge> 0 \<and> b1 \<ge> 0 \<and> a1 + b1 = 10)\<^sub>e \<up> vu\<^sup>>"
-  by (expr_simp_banks add: Loc1_def V1_def ExSys_def)
+  by (pred_auto_banks add: Loc1_def V1_def ExSys_def)
 
 definition Loc2 where "Loc2 = L V2 ExSys"
 
 lemma localise_v2 : "Loc2 = (c2 \<ge> 5 \<and> c2 \<le> 10)\<^sub>e \<up> vu\<^sup>>"
-  apply (expr_simp_banks add: Loc2_def V2_def ExSys_def)
+  apply (pred_auto_banks add: Loc2_def V2_def ExSys_def)
   by presburger
 
 definition Loc3 where "Loc3 = L V3 ExSys"
-
-(*
-definition Loc3_one_alpha where "Loc3_one_alpha = L_one_alpha V3 ExSys_one_alpha"
-
-definition Loc3_two_delta where "Loc3_two_delta = L_two_delta V3 ExSys_two_delta"
-*)
 
 lemma localise_v3 : "Loc3 = (
     (d3 \<ge> 0 \<and> d3 < 5 \<and> e3 = 0)
    \<or>(d3 \<ge> 5 \<and> d3 \<le> 10 \<and> e3 = 1)
   )\<^sub>e \<up> vu\<^sup>>"
-  apply (expr_simp_banks add: Loc3_def V3_def ExSys_def)
-  apply presburger+
-  done
-
-(*
-lemma localise_v3_two_delta : "Loc3_two_delta = 
- \<Delta> ((vu:d3 \<ge> 0 \<and> vu:d3 < 5 \<and> vu:e3 = 0)
-   \<or>(vu:d3 \<ge> 5 \<and> vu:d3 \<le> 10 \<and> vu:e3 = 1))\<^sub>e"
-  apply (expr_simp_banks add: Loc3_two_delta_def V3_def ExSys_two_delta_def L_two_delta_def)
-  apply presburger+
-  done
-
-lemma localise_v3_one_alpha : "Loc3_one_alpha = (
-    (vu:d3 \<ge> 0 \<and> vu:d3 < 5 \<and> vu:e3 = 0)
-   \<or>(vu:d3 \<ge> 5 \<and> vu:d3 \<le> 10 \<and> vu:e3 = 1)
-  )\<^sub>e"
-  apply (expr_simp_banks add: Loc3_one_alpha_def V3_def ExSys_one_alpha_def L_one_alpha_def)
-  apply presburger+
-  done
-*)
+  apply (pred_auto_banks add: Loc3_def V3_def ExSys_def)
+  by presburger+
 
 lemma "(G V1 Loc1) =  (x \<ge> 0 \<and> y \<ge> 0 \<and> x + y = 10)\<^sub>e \<up> sys\<^sup>>"
-  by (expr_simp_banks add: G_def Loc1_def V1_def ExSys_def)
+  by (pred_auto_banks add: Loc1_def V1_def ExSys_def)
 
 lemma "(G V2 Loc2) =  ((max x y \<ge> 5) \<and> (max x y \<le> 10))\<^sub>e  \<up> sys\<^sup>>"
-  apply (expr_simp_banks add: G_def Loc2_def V2_def ExSys_def)
+  apply (pred_auto_banks add: Loc2_def V2_def ExSys_def)
   by presburger
 
-lemma "(G V3 Loc3) =  ( if x < y then x \<ge> 0 \<and> x < 5 else x \<ge> 5 \<and> x \<le> 10)\<^sub>e  \<up> sys\<^sup>>"
-  apply (expr_simp_banks add: G_def Loc3_def V3_def ExSys_def)
-  by presburger
+lemma "(G V3 Loc3) =  ( if x < y then (x \<ge> 0 \<and> x < 5) else (x \<ge> 5 \<and> x \<le> 10))\<^sub>e  \<up> sys\<^sup>>"
+  apply (pred_auto_banks add: Loc3_def V3_def ExSys_def)
+  by presburger+
 
 end
